Initial cleanup of logic directory

src/theory/program_logic/abstract_hoare_logicScript.sml
@@ -4,53 +4,92 @@ open bir_auxiliaryLib;
 
 open bir_auxiliaryTheory;
 
-open abstract_hoare_logic_auxTheory;
+open transition_systemTheory;
 
-val _ = new_theory "abstract_hoare_logic";
+val _ = new_theory "total_program_logic";
 
 (* Judgment of the total-correctness logic *)
-val abstract_jgmt_def = Define `
-  abstract_jgmt m (l:'a) (ls:'a->bool) pre post =
-  !ms .
-   ((m.pc ms) = l) ==> (pre ms) ==>
-   ?ms'. ((m.weak ms ls ms') /\
-    (post ms'))
-`;
+Definition t_jgmt_def:
+ t_jgmt TS (l:'a) (ls:'a->bool) pre post =
+  !s.
+   TS.ctrl s = l ==>
+   pre s ==>
+   ?s'. TS.weak s ls s' /\ post s'
+End
+
+(* Judgment of the total-correctness logic, adjusted for
+ * non-determinism *)
+Definition t_nondet_jgmt_def:
+ t_nondet_jgmt TS (l:'a) (ls:'a->bool) pre post =
+  !s.
+   TS.ctrl s = l ==>
+   pre s ==>
+   TS.weak s ls <> {} /\ (!s'. TS.weak s ls s' /\ post s')
+End
+
 
 (* TODO: Can this be rephrased better?
  * Antecedents guarantee swapping transition system of ANY contract. *)
-val abstract_weak_model_comp_rule_thm = store_thm("abstract_weak_model_comp_rule_thm",
-  ``!m n l ls pre post.
-    weak_model m ==>
-    weak_model n ==>
-    (!ms ls ms'. m.weak ms ls ms' ==> n.weak ms ls ms') ==>
-    (!ms l. (n.pc ms = l)  ==> (m.pc ms = l)) ==>
-    abstract_jgmt m l ls pre post ==>
-    abstract_jgmt n l ls pre post``,
+Theorem total_comp_rule_thm:
+ !TS TS'.
+  first_enc TS ==>
+  first_enc TS' ==>
+  (!s ls s'. TS.weak s ls s' ==> TS'.weak s ls s') ==>
+  (!s l. (TS'.ctrl s = l)  ==> (TS.ctrl s = l)) ==>
+  !l ls pre post.
+   t_jgmt TS l ls pre post ==>
+   t_jgmt TS' l ls pre post
+Proof
+rpt strip_tac >>
+fs [t_jgmt_def] >>
+rpt strip_tac >>
+QSPECL_X_ASSUM ``!s. _`` [`s`] >>
+QSPECL_X_ASSUM ``!s. _`` [`s`] >>
+rfs [] >>
+fs [] >>
+QSPECL_X_ASSUM ``!s ls s'. _`` [`s`, `ls`, `s'`] >>
+rfs [] >>
+Q.EXISTS_TAC `s'` >>
+fs []
+QED
 
-REPEAT STRIP_TAC >>
-FULL_SIMP_TAC std_ss [abstract_jgmt_def] >>
-REPEAT STRIP_TAC >>
-QSPECL_X_ASSUM ``!ms. _`` [`ms`] >>
-QSPECL_X_ASSUM ``!ms. _`` [`ms`] >>
-REV_FULL_SIMP_TAC std_ss [] >>
-FULL_SIMP_TAC std_ss [] >>
-QSPECL_X_ASSUM ``!ms ls ms'. _`` [`ms`, `ls`, `ms'`] >>
-REV_FULL_SIMP_TAC std_ss [] >>
-Q.EXISTS_TAC `ms'` >>
-FULL_SIMP_TAC std_ss []
-);
+Theorem total_nondet_comp_rule_thm:
+ !TS TS'.
+  first_enc TS ==>
+  first_enc TS' ==>
+  (!s ls s'. TS.weak s ls s' ==> TS'.weak s ls s') ==>
+  (!s l. (TS'.ctrl s = l)  ==> (TS.ctrl s = l)) ==>
+  !l ls pre post.
+   t_nondet_jgmt TS l ls pre post ==>
+   t_nondet_jgmt TS' l ls pre post
+Proof
+rpt strip_tac >>
+fs [t_nondet_jgmt_def] >>
+rpt strip_tac >> (
+ QSPECL_X_ASSUM ``!s. _`` [`s`] >>
+ QSPECL_X_ASSUM ``!s. _`` [`s`] >>
+ subgoal `TS'.weak s ls <> {}` >- (
+  gs [GSYM pred_setTheory.MEMBER_NOT_EMPTY] >>
+  QSPECL_X_ASSUM ``!s'. _`` [`s'`] >>
+  gs [] >>
+  res_tac >>
+  metis_tac [pred_setTheory.MEMBER_NOT_EMPTY, pred_setTheory.IN_APP]
+  cheat
+ ) >>
+ gs []
 
+)
+QED
 
 val abstract_case_rule_thm = prove(``
 !m l ls pre post C1.
-  abstract_jgmt m l ls (\ms. (pre ms) /\ (C1 ms)) post ==>
-  abstract_jgmt m l ls (\ms. (pre ms) /\ (~(C1 ms))) post ==>
-  abstract_jgmt m l ls pre post
+  t_jgmt m l ls (\ms. (pre ms) /\ (C1 ms)) post ==>
+  t_jgmt m l ls (\ms. (pre ms) /\ (~(C1 ms))) post ==>
+  t_jgmt m l ls pre post
 ``,
 
 rpt strip_tac >>
-fs [abstract_jgmt_def] >>
+fs [t_jgmt_def] >>
 metis_tac []
 );
 
@@ -61,12 +100,12 @@ val abstract_conseq_rule_thm =
     weak_model m ==>
     (!ms. ((m.pc ms) = l) ==> (pre2 ms) ==> (pre1 ms)) ==>
     (!ms. ((m.pc ms) IN ls) ==> (post1 ms) ==> (post2 ms)) ==>
-    abstract_jgmt m l ls pre1 post1 ==>
-    abstract_jgmt m l ls pre2 post2
+    t_jgmt m l ls pre1 post1 ==>
+    t_jgmt m l ls pre2 post2
   ``,
 
 rpt strip_tac >>
-fs [abstract_jgmt_def] >>
+fs [t_jgmt_def] >>
 metis_tac [weak_pc_in_thm]
 );
 
@@ -77,12 +116,12 @@ val abstract_subset_rule_thm =
   ``!m.  ! l ls1 ls2 pre post .
     weak_model m ==>
     (!ms. ((post ms) ==> (~((m.pc ms) IN ls2)))) ==>
-    abstract_jgmt m l (ls1 UNION ls2) pre post ==>
-    abstract_jgmt m l ls1 pre post``,
+    t_jgmt m l (ls1 UNION ls2) pre post ==>
+    t_jgmt m l ls1 pre post``,
 
-REPEAT STRIP_TAC >>
-REV_FULL_SIMP_TAC std_ss [abstract_jgmt_def] >>
-REPEAT STRIP_TAC >>
+rpt strip_tac >>
+REV_FULL_SIMP_TAC std_ss [t_jgmt_def] >>
+rpt strip_tac >>
 QSPECL_X_ASSUM ``!ms. _`` [`ms`] >>
 METIS_TAC [weak_union_pc_not_in_thm]
 );
@@ -91,18 +130,18 @@ METIS_TAC [weak_union_pc_not_in_thm]
 val abstract_seq_rule_thm = store_thm("abstract_seq_rule_thm",
   ``!m l ls1 ls2 pre post.
     weak_model m ==>
-    abstract_jgmt m l (ls1 UNION ls2) pre post ==>
+    t_jgmt m l (ls1 UNION ls2) pre post ==>
     (!l1.
      l1 IN ls1 ==>
-     abstract_jgmt m l1 ls2 post post
+     t_jgmt m l1 ls2 post post
     ) ==>
-    abstract_jgmt m l ls2 pre post``,
+    t_jgmt m l ls2 pre post``,
 
-REPEAT STRIP_TAC >>
-SIMP_TAC std_ss [abstract_jgmt_def] >>
-REPEAT STRIP_TAC >>
-PAT_X_ASSUM ``abstract_jgmt m l (ls1 UNION ls2) pre post``
-              (fn thm => ASSUME_TAC (SIMP_RULE std_ss [abstract_jgmt_def] thm)) >>
+rpt strip_tac >>
+SIMP_TAC std_ss [t_jgmt_def] >>
+rpt strip_tac >>
+PAT_X_ASSUM ``t_jgmt m l (ls1 UNION ls2) pre post``
+              (fn thm => ASSUME_TAC (SIMP_RULE std_ss [t_jgmt_def] thm)) >>
 QSPECL_X_ASSUM ``!ms. _`` [`ms`] >>
 REV_FULL_SIMP_TAC std_ss [] >>
 Cases_on `m.pc ms' IN ls2` >- (
@@ -112,7 +151,7 @@ subgoal `m.pc ms' IN ls1` >- (
   METIS_TAC [weak_union_thm, weak_pc_in_thm]
 ) >>
 QSPECL_X_ASSUM  ``!l1. _`` [`m.pc ms'`] >>
-REV_FULL_SIMP_TAC std_ss [abstract_jgmt_def] >>
+REV_FULL_SIMP_TAC std_ss [t_jgmt_def] >>
 QSPECL_X_ASSUM  ``!m. _`` [`ms'`] >>
 REV_FULL_SIMP_TAC std_ss [] >>
 ASSUME_TAC (Q.SPECL [`m`] weak_comp_thm) >>
@@ -124,13 +163,13 @@ val abstract_conj_rule_thm = prove(``
   !m.
   weak_model m ==>
   !l ls pre post1 post2.
-  abstract_jgmt m l ls pre post1 ==>
-  abstract_jgmt m l ls pre post2 ==>
-  abstract_jgmt m l ls pre (\ms. (post1 ms) /\ (post2 ms))``,
+  t_jgmt m l ls pre post1 ==>
+  t_jgmt m l ls pre post2 ==>
+  t_jgmt m l ls pre (\ms. (post1 ms) /\ (post2 ms))``,
 
-REPEAT STRIP_TAC >>
-FULL_SIMP_TAC std_ss [abstract_jgmt_def] >>
-REPEAT STRIP_TAC >>
+rpt strip_tac >>
+FULL_SIMP_TAC std_ss [t_jgmt_def] >>
+rpt strip_tac >>
 METIS_TAC [weak_unique_thm]
 );
 
@@ -160,7 +199,7 @@ Defn.tgoal loop_fun_defn
 val (loop_fun_eqns, loop_fun_ind) = Defn.tprove(loop_fun_defn,
   FULL_SIMP_TAC std_ss [loop_step_def] >>
   WF_REL_TAC `measure (\(m,ms,var,l,le,invariant,C1). var ms)` >>
-  REPEAT STRIP_TAC >>
+  rpt strip_tac >>
   REV_FULL_SIMP_TAC std_ss [LET_DEF] >>
   Q.ABBREV_TAC `MS' =  (\ms'.
                m.weak ms ({l} UNION le) ms' /\ (invariant ms /\ C1 ms) /\
@@ -174,7 +213,7 @@ val (loop_fun_eqns, loop_fun_ind) = Defn.tprove(loop_fun_defn,
 val abstract_loop_jgmt_def = Define `
   abstract_loop_jgmt m l le invariant C1 var =
     (~(l IN le) /\
-    !x. abstract_jgmt m l ({l} UNION le) (\ms. invariant ms /\ C1 ms /\ var ms = x:num)
+    !x. t_jgmt m l ({l} UNION le) (\ms. invariant ms /\ C1 ms /\ var ms = x:num)
           (\ms. m.pc ms = l /\ invariant ms /\ var ms < x /\ var ms >= 0))
 `;
 
@@ -185,7 +224,7 @@ val loop_fun_ind_spec =
   Q.SPEC `\m ms var l le invariant C1.
 	   weak_model m ==>
 	   abstract_loop_jgmt m l le invariant C1 var ==>
-	   abstract_jgmt m l le (\ms. invariant ms /\ ~C1 ms) post ==>
+	   t_jgmt m l le (\ms. invariant ms /\ ~C1 ms) post ==>
 	   (invariant ms /\ m.pc ms = l) ==>
 	   (?ms'. m.weak ms le ms' /\ post ms')` loop_fun_ind;
 
@@ -201,7 +240,7 @@ rpt strip_tac >>
 fs [] >>
 rpt strip_tac >>
 Cases_on `~C1 ms` >- (
-  fs [abstract_jgmt_def]
+  fs [t_jgmt_def]
 ) >>
 (* We first prove that one iteration works (first antecedent of induction hypothesis):
  * OK since C1 holds in ms, then use loop judgment to obtain
@@ -210,7 +249,7 @@ subgoal `loop_step m ms var l le invariant C1 <> {}` >- (
   simp [loop_step_def, LET_DEF] >>
   fs [abstract_loop_jgmt_def] >>
   QSPECL_X_ASSUM ``!x. _`` [`(var ms):num`] >>
-  fs [abstract_jgmt_def] >>
+  fs [t_jgmt_def] >>
   QSPECL_X_ASSUM ``!ms. _`` [`ms`] >>
   rfs [] >>
   fs [GSYM pred_setTheory.MEMBER_NOT_EMPTY] >>
@@ -255,10 +294,10 @@ val abstract_loop_rule_thm = store_thm("abstract_loop_rule_thm",
     weak_model m ==>
     !l le invariant C1 var post.
     abstract_loop_jgmt m l le invariant C1 var ==>
-    abstract_jgmt m l le (\ms. invariant ms /\ ~C1 ms) post ==>
-    abstract_jgmt m l le invariant post``,
+    t_jgmt m l le (\ms. invariant ms /\ ~C1 ms) post ==>
+    t_jgmt m l le invariant post``,
 
-metis_tac [abstract_jgmt_def, abstract_loop_rule_tmp_thm]
+metis_tac [t_jgmt_def, abstract_loop_rule_tmp_thm]
 );
 
 val _ = export_theory();
