src/theory/program_logic/transition_systemScript.sml
@@ -1,0 +1,1129 @@
+open HolKernel boolLib bossLib BasicProvers dep_rewrite;
+
+open bir_auxiliaryLib;
+
+open bir_auxiliaryTheory;
+
+val _ = new_theory "transition_system";
+
+(* Transition system *)
+Datatype:
+ transition_system_t =
+  <|(* Transition function *)
+    trs : 'a -> 'a option;
+    (* Weak transition relation *)
+    weak : ('b -> bool) -> 'a -> 'a -> bool;
+    (* A function to obtain the control state from a state.
+     * This allows for isolating parts of the state that
+     * the weak transition is provably oblivious to. *)
+    ctrl : 'a -> 'b
+   |>
+End
+
+(* A weak transition in a transition system is first-encounter
+ * if this property is fulfilled. *)
+Definition first_enc_def:
+ first_enc TS =
+  !s ls s'. TS.weak ls s s' =
+   ?n.
+    (n > 0 /\
+     FUNPOW_OPT TS.trs n s = SOME s' /\
+     TS.ctrl s' IN ls
+    ) /\
+    !n'.
+     n' < n /\ n' > 0 ==>
+     ?s''.
+      FUNPOW_OPT TS.trs n' s = SOME s'' /\
+      TS.ctrl s'' NOTIN ls
+End
+
+(* Avoids expanding first_enc_def, but rewrites all weak using
+ * the first_enc assumption without deleting it *)
+val first_enc_weak_tac =
+ PAT_ASSUM ``first_enc TS`` (fn thm => fs [MP (fst $ EQ_IMP_RULE (Q.SPEC `TS` first_enc_def)) thm]);
+val first_enc_weak_goal_tac =
+ PAT_ASSUM ``first_enc TS`` (fn thm => simp [MP (fst $ EQ_IMP_RULE (Q.SPEC `TS` first_enc_def)) thm]);
+
+Theorem weak_comp:
+ !TS.
+  first_enc TS ==>
+  !ls1 ls2 s s' s''.
+   TS.weak (ls1 UNION ls2) s s' ==>
+   TS.ctrl s' NOTIN ls2 ==>
+   TS.weak ls2 s' s'' ==>
+   TS.weak ls2 s s''
+Proof
+rpt strip_tac >>
+first_enc_weak_tac >>
+qexists_tac `n' + n` >>
+gs [] >>
+rpt strip_tac >| [
+ metis_tac [FUNPOW_OPT_ADD_thm, arithmeticTheory.ADD_COMM],
+
+ subgoal `?s''. FUNPOW_OPT TS.trs (n''-n) s' = SOME s''` >- (
+  irule FUNPOW_OPT_prev_EXISTS >>
+  qexistsl_tac [`n'`, `s''`] >>
+  fs []
+ ) >>
+ Cases_on `n'' < n` >- (
+  metis_tac [pred_setTheory.IN_UNION]
+ ) >>
+ Cases_on `n'' = n` >- (
+  metis_tac []
+ ) >>
+ qexists_tac `s'''` >>
+ conj_tac >| [
+  subgoal `n'' > n` >- (
+   fs []
+  ) >>
+  imp_res_tac FUNPOW_OPT_ADD_thm >>
+  gs [arithmeticTheory.SUB_ADD, arithmeticTheory.GREATER_DEF],
+
+  QSPECL_X_ASSUM ``!n'':num. n'' < n' /\ n'' > 0 ==> _`` [`n''-n`] >>
+  gs []
+ ]
+]
+QED
+
+Theorem weak_unique:
+ !TS.
+  first_enc TS ==>
+  !ls s s' s''.
+   TS.weak ls s s' ==>
+   TS.weak ls s s'' ==>
+   s' = s''
+Proof
+rpt strip_tac >>
+first_enc_weak_tac >>
+`n = n'` suffices_by (
+ strip_tac >>
+ fs []
+) >>
+Cases_on `n < n'` >- (
+ QSPECL_X_ASSUM ``!n'':num. n'' < n' /\ n'' > 0 ==> _`` [`n`] >>
+ rfs []
+) >>
+Cases_on `n > n'` >- (
+ QSPECL_X_ASSUM ``!n'':num. n'' < n /\ n'' > 0 ==> _`` [`n'`] >>
+ rfs [] 
+) >>
+fs [] 
+QED
+
+Theorem weak_union:
+ !TS.
+  first_enc TS ==>
+  !ls1 ls2 s s'.
+   TS.weak (ls1 UNION ls2) s s' ==>
+   TS.ctrl s' NOTIN ls1 ==>
+   TS.weak ls2 s s'
+Proof
+rpt strip_tac >>
+first_enc_weak_tac >>
+qexists_tac `n` >>
+metis_tac [pred_setTheory.IN_UNION]
+QED
+
+Theorem weak_union2:
+ !TS.
+  first_enc TS ==>
+  !ls1 ls2 s s'.
+   TS.weak (ls1 UNION ls2) s s' ==>
+   TS.ctrl s' IN ls2 ==>
+   TS.weak ls2 s s'
+Proof
+rpt strip_tac >>
+first_enc_weak_tac >>
+qexists_tac `n` >>
+metis_tac [pred_setTheory.IN_UNION]
+QED
+
+Theorem weak_ctrl_in:
+ !TS.
+  first_enc TS ==>
+  !ls s s'.
+   TS.weak ls s s' ==>
+   TS.ctrl s' IN ls
+Proof
+metis_tac [first_enc_def]
+QED
+
+Theorem weak_union_ctrl_not_in:
+ !TS.
+  first_enc TS ==>
+  !ls1 ls2 s s'.
+   TS.weak (ls1 UNION ls2) s s' ==>
+   TS.ctrl s' NOTIN ls2 ==>
+   TS.weak ls1 s s'
+Proof
+rpt strip_tac >>
+first_enc_weak_tac >>
+metis_tac [pred_setTheory.IN_UNION]
+QED
+
+Definition ominus_def:
+ (ominus NONE _ = NONE) /\
+ (ominus _ NONE = NONE) /\
+ (ominus (SOME (n:num)) (SOME n') = SOME (n - n'))
+End
+
+Theorem weak_superset_thm:
+ !TS.
+  first_enc TS ==>
+  !ls1 ls2 s s'.
+   TS.weak ls1 s s' ==>
+   ?s''. TS.weak (ls1 UNION ls2) s s''
+Proof
+rpt strip_tac >>
+first_enc_weak_tac >>
+Cases_on `(OLEAST n'. ?s''. n' > 0 /\ n' < n /\ FUNPOW_OPT TS.trs n' s = SOME s'' /\ TS.ctrl s'' IN ls2)` >- (
+ fs [] >>
+ qexistsl_tac [`s'`, `n`] >>
+ fs [] >>
+ rpt strip_tac >>
+ fs [whileTheory.OLEAST_EQ_NONE] >>
+ metis_tac []
+) >>
+fs [whileTheory.OLEAST_EQ_SOME] >>
+qexistsl_tac [`s''`, `x`] >>
+fs [] >>
+rpt strip_tac >>
+QSPECL_X_ASSUM  ``!n':num. n' < n /\ n' > 0 ==> _`` [`n''`] >>
+gs [] >>
+QSPECL_X_ASSUM  ``!n':num. n' < x ==> _`` [`n''`] >>
+gs []
+QED
+
+Theorem weak_nonempty:
+ !TS.
+  first_enc TS ==>
+  !s ls. 
+   TS.weak ls s <> {} <=> (?s'. TS.weak ls s s')
+Proof
+rpt strip_tac >>
+fs [GSYM pred_setTheory.MEMBER_NOT_EMPTY] >>
+eq_tac >> (rpt strip_tac) >| [
+ qexists_tac `x` >>
+ fs [pred_setTheory.IN_APP],
+
+ qexists_tac `s'` >>
+ fs [pred_setTheory.IN_APP]
+]
+QED
+
+Theorem weak_inter:
+ !TS.
+  first_enc TS ==>
+  !s s' s'' ls1 ls2.
+   DISJOINT ls1 ls2 ==>
+   TS.weak ls2 s s' ==>
+   TS.weak (ls1 UNION ls2) s s'' ==>
+   TS.ctrl s'' IN ls1 ==>
+   TS.weak ls2 s'' s'
+Proof
+rpt strip_tac >>
+(* s goes to s' in n steps. s goes to s'' in n' steps, for which:
+ * n'>n: impossible, by the first-encounter property
+ * n=n': impossible, since s' is in ls2 and s'' is in ls1 (disjoint sets)
+ * n'<n: then s' can be reached by taking n'-n steps, with no ls2-encounters
+ * in-between *)
+first_enc_weak_tac >>
+subgoal `~(n'>n)` >- (
+ QSPECL_X_ASSUM ``!n'':num. n'' < n' /\ n'' > 0 ==> _`` [`n`] >>
+ gs []
+) >>
+subgoal `~(n'=n)` >- (
+ strip_tac >>
+ gs [] >>
+ metis_tac [pred_setTheory.IN_DISJOINT]
+) >>
+subgoal `n'<n` >- (
+ fs []
+) >>
+qexists_tac `n-n'` >>
+rpt strip_tac >| [
+ fs [],
+
+ (* by combining execution *)
+ irule FUNPOW_OPT_split2 >>
+ fs [] >>
+ qexists_tac `s` >>
+ fs [],
+
+ (* non-encounter in earlier steps *)
+ QSPECL_X_ASSUM ``!n':num. n' < n /\ n' > 0 ==> _`` [`n' + n''`] >>
+ gs [] >>
+ qexists_tac `s'''` >>
+ fs [] >>
+ metis_tac [FUNPOW_OPT_INTER, arithmeticTheory.ADD_COMM]
+]
+QED
+
+Theorem weak_least_trs:
+ !TS.
+  first_enc TS ==>
+  !s ls s'.
+   s <> s' ==>
+   TS.weak ls s s' ==>
+   ?n'. n' > 0 /\ (OLEAST n'. FUNPOW_OPT TS.trs n' s = SOME s') = SOME n'
+Proof
+rpt strip_tac >>
+first_enc_weak_tac >>
+qexists_tac `n` >>
+fs [whileTheory.OLEAST_EQ_SOME] >>
+rpt strip_tac >>
+QSPECL_X_ASSUM ``!n'. _`` [`n'`] >>
+gs [] >>
+subgoal `n' = 0` >- (
+ fs []
+) >>
+rw [] >>
+gs [FUNPOW_OPT_compute]
+QED
+
+Theorem weak_union_ctrl:
+ !TS.
+  first_enc TS ==>
+  !ls1 ls2 s s' s''.
+   TS.weak ls2 s s' ==>
+   TS.weak (ls1 UNION ls2) s s'' ==>
+   s' <> s'' ==>
+   TS.ctrl s'' IN ls1
+Proof
+rpt strip_tac >>
+first_enc_weak_tac >>
+Cases_on `n' > n` >- (
+ QSPECL_X_ASSUM ``!n'':num. n'' < n' /\ n'' > 0 ==> _`` [`n`] >>
+ gs []
+) >>
+Cases_on `n' = n` >- (
+ gs []
+) >>
+QSPECL_X_ASSUM ``!n':num. n' < n /\ n' > 0 ==> _`` [`n'`] >>
+gs []
+QED
+
+Theorem weak_subset:
+ !TS.
+  first_enc TS ==>
+  !ls1 ls2 s s'.
+   TS.weak (ls1 UNION ls2) s s' ==>
+   ls1 SUBSET ls2 ==>
+   TS.weak ls2 s s'
+Proof
+rpt strip_tac >>
+fs [pred_setTheory.SUBSET_UNION_ABSORPTION]
+QED
+
+
+(****************************)
+(* Weak transition function *)
+(****************************)
+
+(* This is a non-executable function that computes a state (Hilbert's choice of one)
+ * that is related to the given initial state by weak to ls. *)
+Definition weak_exec_def:
+ weak_exec TS ls s =
+  let
+   S' = TS.weak ls s
+  in
+   if S' = {}
+   then NONE
+   else SOME (CHOICE S')
+End
+
+(* The above, applied multiple times *)
+Definition weak_exec_n_def:
+ weak_exec_n TS s ls n = FUNPOW_OPT (weak_exec TS ls) n s
+End
+
+Theorem weak_exec_exists:
+ !TS.
+  first_enc TS ==>
+  !ls s s'.
+  TS.weak ls s s' <=> weak_exec TS ls s = SOME s'
+Proof
+rpt strip_tac >>
+fs [weak_exec_def] >>
+eq_tac >> (
+ strip_tac
+) >| [
+ subgoal `TS.weak ls s = {s'}` >- (
+  fs [GSYM pred_setTheory.UNIQUE_MEMBER_SING, pred_setTheory.IN_APP] >>
+  metis_tac [weak_unique]
+ ) >>
+ fs [],
+
+ metis_tac [pred_setTheory.CHOICE_DEF, pred_setTheory.IN_APP]
+]
+QED
+
+(* TODO: Replace weak with weak_exec_n of 1 in the below? *)
+
+Theorem weak_exec_to_n:
+  !TS ls s s'. 
+   weak_exec TS ls s = SOME s' <=>
+   weak_exec_n TS s ls 1 = SOME s'
+Proof
+rpt strip_tac >>
+fs [weak_exec_n_def, FUNPOW_OPT_def]
+QED
+
+Theorem weak_exec_n_prev:
+ !TS ls s s' n_l.
+  weak_exec_n TS s ls (SUC n_l) = SOME s' ==>
+  ?s''. weak_exec_n TS s ls n_l = SOME s'' /\ weak_exec_n TS s'' ls 1 = SOME s'
+Proof
+rpt strip_tac >>
+fs [weak_exec_n_def] >>
+subgoal `SUC n_l > 0` >- (
+ fs []
+) >>
+imp_res_tac FUNPOW_OPT_prev_EXISTS >>
+QSPECL_X_ASSUM ``!n'. _`` [`n_l`] >>
+fs [] >>
+Cases_on `n_l = 0` >- (
+ gs [FUNPOW_OPT_compute]
+) >>
+irule FUNPOW_OPT_split >>
+qexistsl_tac [`SUC n_l`, `s`] >>
+fs [arithmeticTheory.ADD1]
+QED
+
+(* TODO: Useful?
+Theorem weak_exec_n_split:
+!m. first_enc m ==>
+!s s' s'' ls n n'.
+n > n' ==>
+weak_exec_n m s ls n = SOME s' ==>
+weak_exec_n m s ls (n - n') = SOME s'' ==>
+weak_exec_n m s'' ls n' = SOME s'
+Proof
+cheat
+QED
+*)
+
+Theorem weak_exec_n_split2:
+ !TS ls s s' s'' n n'.
+   n >= n' ==>
+   weak_exec_n TS s ls n' = SOME s'' ==>
+   weak_exec_n TS s ls n = SOME s' ==>
+   weak_exec_n TS s'' ls (n - n') = SOME s'
+Proof
+rpt strip_tac >>
+fs [weak_exec_n_def] >>
+Cases_on `n = n'` >- (
+ fs [FUNPOW_OPT_compute]
+) >>
+subgoal `n > n'` >- (
+ fs []
+) >>
+metis_tac [FUNPOW_SUB, FUNPOW_OPT_def, arithmeticTheory.FUNPOW_ADD]
+QED
+
+
+Theorem weak_exec_n_cycle:
+ !TS s s' ls n_l n_l'.
+ n_l > 0 /\ weak_exec_n TS s ls n_l = SOME s ==>
+ s <> s' ==>
+ (OLEAST n_l'. weak_exec_n TS s ls n_l' = SOME s') = SOME n_l' ==>
+ n_l' < n_l
+Proof
+rpt strip_tac >>
+CCONTR_TAC >>
+Cases_on `n_l' = n_l` >- (
+ fs [whileTheory.OLEAST_EQ_SOME]
+) >>
+subgoal `n_l' > n_l` >- (
+ gs []
+) >>
+subgoal `weak_exec_n TS s ls (n_l' - n_l) = SOME s'` >- (
+ irule weak_exec_n_split2 >>
+ fs [whileTheory.OLEAST_EQ_SOME] >>
+ qexists_tac `s` >>
+ fs []
+) >>
+fs [whileTheory.OLEAST_EQ_SOME] >>
+QSPECL_X_ASSUM ``!n_l''. n_l'' < n_l' ==> weak_exec_n TS s ls n_l'' <> SOME s'`` [`n_l' - n_l`] >>
+gs []
+QED
+
+(* TODO: Technically, this doesn't need OLEAST for the encounter of s'
+ * Let this rely on sub-lemma for incrementing weak_exec_n instead
+ * of reasoning on FUNPOW_OPT *)
+Theorem weak_exec_incr_last:
+ !TS.
+ first_enc TS ==>
+ !s ls s' n_l s''.
+ (OLEAST n. weak_exec_n TS s ls n = SOME s') = SOME n_l ==>
+ TS.weak ls s' s'' ==>
+ weak_exec_n TS s ls (SUC n_l) = SOME s''
+Proof
+rpt strip_tac >>
+simp [weak_exec_n_def, arithmeticTheory.ADD1] >>
+ONCE_REWRITE_TAC [arithmeticTheory.ADD_SYM] >>
+irule FUNPOW_OPT_ADD_thm >>
+qexists_tac `s'` >>
+fs [whileTheory.OLEAST_EQ_SOME, weak_exec_n_def] >>
+simp [FUNPOW_OPT_def] >>
+metis_tac [weak_exec_exists]
+QED
+
+Theorem weak_exec_incr_first:
+ !TS.
+ first_enc TS ==>
+ !s ls s' n_l s''.
+ TS.weak ls s s' ==>
+ (OLEAST n. weak_exec_n TS s' ls n = SOME s'') = SOME n_l ==>
+ weak_exec_n TS s ls (SUC n_l) = SOME s''
+Proof
+rpt strip_tac >>
+simp [weak_exec_n_def, arithmeticTheory.ADD1] >>
+irule FUNPOW_OPT_ADD_thm >>
+qexists_tac `s'` >>
+fs [whileTheory.OLEAST_EQ_SOME, weak_exec_n_def] >>
+simp [FUNPOW_OPT_def] >>
+metis_tac [weak_exec_exists]
+QED
+
+Theorem weak_exec_n_add:
+ !TS s s' s'' ls n n'.
+ weak_exec_n TS s ls n = SOME s' ==>
+ weak_exec_n TS s' ls n' = SOME s'' ==>
+ weak_exec_n TS s ls (n + n') = SOME s''
+Proof
+rpt strip_tac >>
+fs [weak_exec_n_def] >>
+metis_tac [FUNPOW_OPT_ADD_thm, arithmeticTheory.ADD_COMM]
+QED
+
+Theorem weak_exec_n_inter:
+ !TS.
+ first_enc TS ==>
+ !s s' ls1 ls2 n_l n_l'.
+ DISJOINT ls1 ls2 ==>
+ weak_exec_n TS s ls2 1 = SOME s' ==>
+ (OLEAST n_l. weak_exec_n TS s (ls1 UNION ls2) n_l = SOME s') = SOME n_l ==>
+ n_l' < n_l ==>
+ !s''.
+ (OLEAST n_l. weak_exec_n TS s (ls1 UNION ls2) n_l = SOME s'') = SOME n_l' ==>
+ weak_exec_n TS s'' ls2 1 = SOME s'
+Proof
+ntac 7 strip_tac >>
+Induct_on `n_l'` >- (
+ rpt strip_tac >>
+ fs [whileTheory.OLEAST_EQ_SOME, weak_exec_n_def, FUNPOW_OPT_compute]
+) >>
+rpt strip_tac >>
+gs [whileTheory.OLEAST_EQ_SOME] >>
+imp_res_tac weak_exec_n_prev >>
+QSPECL_X_ASSUM ``!s'3'.
+          weak_exec_n TS s (ls1 UNION ls2) n_l' = SOME s'3' /\
+          (!n_l.
+             n_l < n_l' ==>
+             weak_exec_n TS s (ls1 UNION ls2) n_l <> SOME s'3') ==>
+          weak_exec_n TS s'3' ls2 1 = SOME s'`` [`s'''`] >>
+gs [] >>
+subgoal `!n_l. n_l < n_l' ==> weak_exec_n TS s (ls1 UNION ls2) n_l <> SOME s'3'` >- (
+ rpt strip_tac >>
+ QSPECL_X_ASSUM ``!n_l.
+          n_l < SUC n_l' ==>
+          weak_exec_n TS s (ls1 UNION ls2) n_l <> SOME s''`` [`SUC n_l''`] >>
+ gs [] >>
+ metis_tac [weak_exec_n_add, arithmeticTheory.ADD1]
+) >>
+fs [GSYM weak_exec_to_n] >>
+PAT_ASSUM ``first_enc TS`` (fn thm => fs [GSYM (HO_MATCH_MP weak_exec_exists thm)]) >>
+irule weak_inter >>
+fs [] >>
+qexistsl_tac [`ls1`, `s'''`] >>
+fs [] >>
+subgoal `s' <> s''` >- (
+QSPECL_X_ASSUM ``!n_l'.
+          n_l' < n_l ==> weak_exec_n TS s (ls1 UNION ls2) n_l' <> SOME s'`` [`SUC n_l'`] >>
+ gs []
+) >>
+metis_tac [weak_union_ctrl]
+QED
+
+Theorem weak_inter_exec:
+ !TS.
+  first_enc TS ==>
+  !ls1 ls2 s n_l s' s''.
+   TS.weak ls2 s s' ==>
+   DISJOINT ls1 ls2 ==>
+   (OLEAST n. weak_exec_n TS s (ls1 UNION ls2) n = SOME s') = SOME n_l ==>
+   SING (\n. n < n_l /\ weak_exec_n TS s (ls1 UNION ls2) n = SOME s'') ==>
+   TS.weak ls2 s'' s'
+Proof
+rpt strip_tac >>
+PAT_ASSUM ``first_enc TS`` (fn thm => fs [HO_MATCH_MP weak_exec_exists thm]) >>
+fs [weak_exec_to_n] >>
+irule weak_exec_n_inter >>
+fs [pred_setTheory.SING_DEF, whileTheory.OLEAST_EQ_SOME] >>
+fs [GSYM pred_setTheory.UNIQUE_MEMBER_SING] >>
+qexistsl_tac [`ls1`, `n_l`, `x`, `s`] >>
+fs [] >>
+rpt strip_tac >>
+QSPECL_X_ASSUM  ``!y. y < n_l /\ weak_exec_n TS s (ls1 UNION ls2) y = SOME s'' ==> x = y`` [`n_l'`] >>
+subgoal `n_l' < n_l` >- (
+ gs []
+) >>
+fs []
+QED
+
+Theorem weak_exec_n_OLEAST_equiv:
+ !TS.
+  first_enc TS ==>
+  !ls s s'.
+   (OLEAST n_l. n_l > 0 /\ weak_exec_n TS s ls n_l = SOME s') = SOME 1 ==>
+   TS.weak ls s s'
+Proof
+rpt strip_tac >>
+fs [whileTheory.OLEAST_EQ_SOME, GSYM weak_exec_to_n] >>
+PAT_ASSUM ``first_enc TS`` (fn thm => fs [GSYM (HO_MATCH_MP weak_exec_exists thm)])
+QED
+
+(* Continuing weak_exec_n at s'', intermediately between s and s'' *)
+Theorem weak_exec_n_OLEAST_inter:
+ !TS.
+  first_enc TS ==>
+  !s s' s'' ls n' n'' n_l.
+  (OLEAST n'. FUNPOW_OPT TS.trs n' s = SOME s') = SOME n' ==>
+  (OLEAST n''. n'' > 0 /\ FUNPOW_OPT TS.trs n'' s = SOME s'') = SOME n'' ==>
+  n' > n'' ==>
+  (OLEAST n_l. n_l > 0 /\ weak_exec_n TS s ls n_l = SOME s'') = SOME 1 ==>
+  (OLEAST n_l. weak_exec_n TS s'' ls n_l = SOME s') = SOME n_l ==>
+  (OLEAST n_l. weak_exec_n TS s ls n_l = SOME s') = SOME (n_l + 1)
+Proof
+rpt strip_tac >>
+simp [whileTheory.OLEAST_EQ_SOME] >>
+conj_tac >| [
+ metis_tac [arithmeticTheory.ADD1, weak_exec_incr_first, weak_exec_n_OLEAST_equiv],
+
+ fs [whileTheory.OLEAST_EQ_SOME] >>
+ subgoal `s <> s'` >- (
+  QSPECL_X_ASSUM ``!n''. n'' < n' ==> FUNPOW_OPT TS.trs n'' s <> SOME s'`` [`0`] >>
+  subgoal `0 < n'` >- (
+   fs []
+  ) >>
+  gs [FUNPOW_OPT_compute]
+ ) >>
+ subgoal `s'' <> s'` >- (
+  QSPECL_X_ASSUM ``!n''. n'' < n' ==> FUNPOW_OPT TS.trs n'' s <> SOME s'`` [`n''`] >>
+  gs []
+ ) >>
+ subgoal `n_l > 0` >- (
+  Cases_on `n_l = 0` >- (
+   fs [weak_exec_n_def, FUNPOW_OPT_compute]
+  ) >>
+  fs []
+ ) >>
+ `weak_exec_n TS s ls 1 <> SOME s' /\ !n_l'. n_l' < n_l ==> weak_exec_n TS s'' ls n_l' <> SOME s'` suffices_by (
+  rpt strip_tac >>
+  fs [] >>
+  QSPECL_X_ASSUM ``!n_l'. n_l' < n_l ==> weak_exec_n TS s'' ls n_l' <> SOME s'`` [`n_l' - 1`] >>
+  gs [] >>
+  subgoal `n_l' >= 1` >- (
+   Cases_on `n_l' = 0` >- (
+    fs [weak_exec_n_def, FUNPOW_OPT_compute]
+   ) >>
+   fs []
+  ) >>
+  metis_tac [weak_exec_n_split2]
+ ) >>
+ QSPECL_X_ASSUM ``!n''. n'' < n' ==> FUNPOW_OPT TS.trs n'' s <> SOME s'`` [`n''`] >>
+ gs [] 
+]
+QED
+
+Theorem weak_exec_1_superset_lemma:
+ !TS.
+  first_enc TS ==>
+  !ls1 ls2 s'.
+   !n n'. n' <= n ==>
+          n' >= 1 ==>
+          !s. TS.weak ls1 s s' /\ ((OLEAST n'. FUNPOW_OPT TS.trs n' s = SOME s') = SOME n') ==>
+          s <> s' ==>
+          ls1 SUBSET ls2 ==>
+          ?n_l. n_l >= 1 /\ (OLEAST n_l. weak_exec_n TS s ls2 n_l = SOME s') = SOME n_l
+Proof
+ntac 5 strip_tac >>
+Induct_on `n` >- (
+ fs []
+) >>
+rpt strip_tac >>
+Cases_on `n' < SUC n` >- (
+ QSPECL_X_ASSUM ``!n'. _`` [`n'`] >>
+ gs []
+) >>
+subgoal `n' = SUC n` >- (
+ fs [] 
+) >>
+Cases_on `n = 0` >- (
+ gs [] >>
+ subgoal `n' = 1` >- (
+  fs [] 
+ ) >>
+ fs [whileTheory.OLEAST_EQ_SOME] >>
+ qexists_tac `1` >>
+ fs [] >>
+ conj_tac >| [
+  fs [GSYM weak_exec_to_n] >>
+  PAT_ASSUM ``first_enc TS`` (fn thm => fs [GSYM (HO_MATCH_MP weak_exec_exists thm)]) >>
+  first_enc_weak_tac >>
+  qexists_tac `1` >>
+  fs [] >>
+  metis_tac [weak_ctrl_in, pred_setTheory.SUBSET_THM],
+
+  rpt strip_tac >>
+  subgoal `n_l' = 0` >- (
+   fs [] 
+  ) >>
+  fs [weak_exec_n_def, FUNPOW_OPT_compute]
+ ]
+) >>
+(* 1. There exists a state s'' which we go to with weak-ls2 from s. (weak_superset_thm should suffice)
+ * s'' is reached with more trs than s': contradiction.
+ * s'' is reached with same amount of trs as s': s'' is s', proof completed
+ * with witness n_l''.
+ * s'' is reached with fewer trs than s': use induction hypothesis specialised for s'', then add
+ * numbers of weak-ls2 transitions together for the witness. *)
+subgoal `?s''. (OLEAST n_l''. n_l'' > 0 /\ weak_exec_n TS s ls2 n_l'' = SOME s'') = SOME 1` >- (
+ subgoal `?s''. TS.weak (ls1 UNION ls2) s s''` >- (
+  metis_tac [weak_superset_thm]
+ ) >>
+ qexistsl_tac [`s''`] >>
+ fs [whileTheory.OLEAST_EQ_SOME] >>
+ metis_tac [weak_subset, weak_exec_to_n, weak_exec_exists]
+) >>
+subgoal `?n''. (OLEAST n''. n'' > 0 /\ FUNPOW_OPT TS.trs n'' s = SOME s'') = SOME n''` >- (
+ (* Since s'' is reached by non-zero weak transitions, there must be a (least) non-zero number of trs
+  * that reaches it *)
+ fs [whileTheory.OLEAST_EQ_SOME] >>
+ fs [GSYM weak_exec_to_n] >>
+ PAT_ASSUM ``first_enc TS`` (fn thm => fs [GSYM (HO_MATCH_MP weak_exec_exists thm)]) >>
+ first_enc_weak_tac >>
+ qexists_tac `n'''` >>
+ fs [] >>
+ rpt strip_tac >>
+ QSPECL_X_ASSUM ``!n':num. n' < n'3' /\ n' > 0 ==> _`` [`n''''`] >>
+ gs []
+) >>
+(* s'' is reached with more trs than s': contradiction, s' would have been crossed *)
+Cases_on `n'' > n'` >- (
+ fs [whileTheory.OLEAST_EQ_SOME] >>
+ subgoal `TS.weak ls2 s s''` >- (
+  metis_tac [weak_exec_to_n, weak_exec_exists]
+ ) >>
+ first_enc_weak_tac >>
+ (* TODO: Make some kind of lemma here? *)
+ Q.SUBGOAL_THEN `n'4' = n''` (fn thm => fs [thm]) >- (
+  Cases_on `n'' < n'4'` >- (
+   QSPECL_X_ASSUM ``!n':num. n' < n'4' /\ n' > 0 ==> _`` [`n''`] >>
+   gs []
+  ) >>
+  Cases_on `n'' > n'4'` >- (
+   QSPECL_X_ASSUM ``!n'3':num. n'3' < n'' ==> _`` [`n''''`] >>
+   gs []
+  ) >>
+  fs []
+ ) >>
+ (* TODO: Make some kind of lemma here? *)
+ Q.SUBGOAL_THEN `n'3' = n'` (fn thm => fs [thm]) >- (
+  Cases_on `n' < n'3'` >- (
+   QSPECL_X_ASSUM ``!n':num. n' < n'3' /\ n' > 0 ==> _`` [`n'`] >>
+   gs []
+  ) >>
+  Cases_on `n' > n'3'` >- (
+   QSPECL_X_ASSUM ``!n':num. n' < n'3' /\ n' > 0 ==> _`` [`n'''`] >>
+   gs []
+  ) >>
+  fs []
+ ) >>
+ QSPECL_X_ASSUM ``!n':num. n' < n'' /\ n' > 0 ==> _`` [`n'`] >>
+ gs [] >>
+ metis_tac [pred_setTheory.SUBSET_THM]
+) >>
+Cases_on `n'' = n'` >- (
+ qexists_tac `1` >>
+ subgoal `s'' = s'` >- (
+  fs [whileTheory.OLEAST_EQ_SOME]
+ ) >>
+ fs [whileTheory.OLEAST_EQ_SOME] >>
+ rpt strip_tac >>
+ subgoal `n_l = 0` >- (
+  fs []
+ ) >>
+ fs [weak_exec_n_def, FUNPOW_OPT_compute]
+) >>
+subgoal `n'' < n'` >- (
+ fs []
+) >>
+QSPECL_X_ASSUM ``!n'. _`` [`n' - n''`] >>
+rfs [] >>
+subgoal `n' <= n + n''` >- (
+ gs [whileTheory.OLEAST_EQ_SOME]
+) >>
+fs [] >>
+QSPECL_X_ASSUM ``!s'''. _`` [`s''`] >>
+
+(* Should be possible to prove with some inter theorem... *)
+subgoal `TS.weak ls1 s'' s'` >- (
+ (* Next state in s'' is s'... *)
+ first_enc_weak_goal_tac >>
+ qexists_tac `n' - n''` >>
+ fs [] >>
+ rpt conj_tac >| [
+  irule FUNPOW_OPT_split >>
+  qexistsl_tac [`n'`, `s`] >>
+  fs [whileTheory.OLEAST_EQ_SOME],
+
+  metis_tac [weak_ctrl_in],
+
+  rpt strip_tac >>
+  fs [whileTheory.OLEAST_EQ_SOME] >>
+  first_enc_weak_tac >>
+  (* TODO: Make some kind of lemma here? *)
+  subgoal `n'''' = n'` >- (
+   Cases_on `n' < n'4'` >- (
+    QSPECL_X_ASSUM ``!n':num. n' < n'4' /\ n' > 0 ==> _`` [`n'`] >>
+    gs []
+   ) >>
+   Cases_on `n' > n'4'` >- (
+    QSPECL_X_ASSUM ``!n'':num. n'' < n' ==> _`` [`n''''`] >>
+    gs []
+   ) >>
+   fs []
+  ) >>
+  gs [] >>
+  QSPECL_X_ASSUM ``!n'5':num. n'5' < n' /\ n'5' > 0 ==> _`` [`n''' + n''`] >>
+  gs [] >>
+  qexists_tac `s'''` >>
+  fs [] >>
+  irule FUNPOW_OPT_split >>
+  qexistsl_tac [`n'' + n'3'`, `s`] >>
+  fs []
+ ]
+) >>
+fs [] >>
+subgoal `(OLEAST n'. FUNPOW_OPT TS.trs n' s'' = SOME s') = SOME (n' - n'')` >- (
+ fs [whileTheory.OLEAST_EQ_SOME] >>
+ conj_tac >| [
+  irule FUNPOW_OPT_split >>
+  qexistsl_tac [`n'`, `s`] >>
+  fs [],
+
+  rpt strip_tac >>
+  QSPECL_X_ASSUM ``!n'':num. n'' < n' ==> _`` [`n'' + n'''`] >>
+  gs [] >>
+  metis_tac [FUNPOW_OPT_ADD_thm, arithmeticTheory.ADD_COMM]
+ ]
+) >>
+fs [] >>
+subgoal `s'' <> s'` >- (
+ (* Since s'' NOTIN ls1, while s' IN ls1 *)
+ first_enc_weak_tac >>
+ (* TODO: Make some kind of lemma here? *)
+ Q.SUBGOAL_THEN `n'3' = n'` (fn thm => fs [thm]) >- (
+  Cases_on `n' < n'3'` >- (
+   QSPECL_X_ASSUM ``!n':num. n' < n'3' /\ n' > 0 ==> _`` [`n'`] >>
+   gs [whileTheory.OLEAST_EQ_SOME]
+  ) >>
+  Cases_on `n' > n'3'` >- (
+   gs [whileTheory.OLEAST_EQ_SOME]
+  ) >>
+  fs []
+ ) >>
+ QSPECL_X_ASSUM ``!n'5':num. n'5' < n' /\ n'5' > 0 ==> _`` [`n''`] >>
+ gs [whileTheory.OLEAST_EQ_SOME] >>
+ strip_tac >>
+ fs []
+) >>
+fs [] >>
+qexists_tac `1 + n_l` >>
+fs [] >>
+irule weak_exec_n_OLEAST_inter >>
+fs [] >>
+qexistsl_tac [`n''`, `s''`] >>
+fs []
+QED
+
+(* TODO: Generalise this *)
+(* TODO: Change weak_exec_n 1 to weak? *)
+Theorem weak_exec_1_superset:
+ !TS.
+  first_enc TS ==>
+  !ls1 ls2 s s'.
+   weak_exec_n TS s ls1 1 = SOME s' ==>
+   s <> s' ==>
+   ls1 SUBSET ls2 ==>
+   ?n. n >= 1 /\ (OLEAST n. weak_exec_n TS s ls2 n = SOME s') = SOME n
+Proof
+rpt strip_tac >>
+fs [GSYM weak_exec_to_n] >>
+PAT_ASSUM ``first_enc TS`` (fn thm => fs [GSYM (HO_MATCH_MP weak_exec_exists thm)]) >>
+subgoal `?n'. n' > 0 /\ (OLEAST n'. FUNPOW_OPT TS.trs n' s = SOME s') = SOME n'` >- (
+ (* Since weak goes from s to s', there must be a least number of primitive transitions such that
+  * s goes to s' *)
+ metis_tac [weak_least_trs]
+) >>
+irule weak_exec_1_superset_lemma >>
+fs [] >>
+rpt strip_tac >| [
+ qexists_tac `n'` >>
+ fs [],
+
+ metis_tac []
+]
+QED
+
+(* TODO: Strengthen conclusion to state either s'' is s', or ctrl is in ls2? *)
+Theorem weak_exec_exists_superset:
+ !TS.
+  first_enc TS ==>
+  !ls1 ls2 s s'. 
+   TS.weak ls1 s s' ==>
+   ?s''. weak_exec TS (ls1 UNION ls2) s = SOME s''
+Proof
+rpt strip_tac >>
+fs [weak_exec_def, weak_nonempty] >>
+metis_tac [weak_superset_thm]
+QED
+
+(* Note: s <> s' used to avoid proving case where least n is zero *)
+Theorem weak_exec_n_exists_superset:
+ !TS.
+  first_enc TS ==>
+  !ls1 ls2 s s'. 
+   TS.weak ls1 s s' ==>
+   s <> s' ==>
+   ?n. (OLEAST n. weak_exec_n TS s (ls1 UNION ls2) n = SOME s') = SOME n
+Proof
+rpt strip_tac >>
+fs [whileTheory.OLEAST_EQ_SOME] >>
+subgoal `weak_exec_n TS s ls1 1 = SOME s'` >- (
+ PAT_ASSUM ``first_enc TS`` (fn thm => fs [HO_MATCH_MP weak_exec_exists thm]) >>
+ fs [weak_exec_to_n]
+) >>
+imp_res_tac weak_exec_1_superset >>
+QSPECL_X_ASSUM ``!ls2. _`` [`ls1 UNION ls2`] >>
+fs [] >>
+qexists_tac `n` >>
+fs [whileTheory.OLEAST_EQ_SOME]
+QED
+
+Theorem weak_exec_least_nonzero:
+ !TS ls s s' n_l.
+ (OLEAST n. weak_exec_n TS s ls n = SOME s') = SOME n_l ==>
+ s <> s' ==>
+ n_l > 0
+Proof
+rpt strip_tac >>
+Cases_on `n_l` >> (
+ fs []
+) >>
+fs [whileTheory.OLEAST_EQ_SOME, weak_exec_n_def, FUNPOW_OPT_def]
+QED
+
+Theorem weak_exec_sing_least_less:
+ !TS ls s s' n_l.
+ SING (\n. n < n_l /\ weak_exec_n TS s ls n = SOME s') ==>
+ ?n_l'. (OLEAST n. weak_exec_n TS s ls n = SOME s') = SOME n_l' /\ n_l' < n_l
+Proof
+rpt strip_tac >>
+fs [pred_setTheory.SING_DEF, whileTheory.OLEAST_EQ_SOME] >>
+qexists_tac `x` >>
+rpt strip_tac >> (
+ fs [GSYM pred_setTheory.UNIQUE_MEMBER_SING]
+) >>
+QSPECL_X_ASSUM ``!y. y < n_l /\ weak_exec_n TS s ls y = SOME s' ==> x = y`` [`n`] >>
+gs []
+QED
+
+
+(* TODO: Technically, this doesn't need OLEAST for the encounter of s' *)
+Theorem weak_exec_incr_least:
+ !TS.
+  first_enc TS ==>
+  !s ls s' s_e n_l n_l' s''.
+   (OLEAST n. weak_exec_n TS s ls n = SOME s_e) = SOME n_l ==>
+   s'' <> s_e ==>
+   (OLEAST n. weak_exec_n TS s ls n = SOME s') = SOME n_l' ==>
+   TS.weak ls s' s'' ==>
+   SING (\n. n < n_l /\ weak_exec_n TS s ls n = SOME s'') ==>
+   n_l' < n_l ==>
+   (OLEAST n. weak_exec_n TS s ls n = SOME s'') = SOME (SUC n_l')
+Proof
+rpt strip_tac >>
+imp_res_tac weak_exec_incr_last >>
+fs [whileTheory.OLEAST_EQ_SOME] >>
+rpt strip_tac >>
+subgoal `SUC n_l' < n_l` >- (
+ Cases_on `SUC n_l' = n_l` >- (
+  fs []
+ ) >>
+ fs []
+) >>
+fs [pred_setTheory.SING_DEF] >>
+fs [GSYM pred_setTheory.UNIQUE_MEMBER_SING] >>
+QSPECL_ASSUM ``!y. y < n_l /\ weak_exec_n TS s ls y = SOME s'' ==> x = y`` [`SUC n_l'`] >>
+QSPECL_X_ASSUM ``!y. y < n_l /\ weak_exec_n TS s ls y = SOME s'' ==> x = y`` [`n`] >>
+gs []
+QED
+
+Theorem weak_exec_uniqueness:
+ !TS.
+ first_enc TS ==>
+ !ls s s' s'' s''' n_l n_l'. 
+ (OLEAST n. weak_exec_n TS s ls n = SOME s') = SOME n_l ==>
+ (OLEAST n. weak_exec_n TS s ls n = SOME s'') = SOME n_l' ==>
+ n_l' < n_l ==>
+ TS.weak ls s'' s''' ==>
+ s''' <> s' ==>
+ SING (\n_l''. n_l'' < n_l /\ weak_exec_n TS s ls n_l'' = SOME s''')
+Proof
+rpt strip_tac >>
+subgoal `weak_exec_n TS s ls (n_l' + 1) = SOME s'3'` >- (
+ irule weak_exec_n_add >>
+ fs [whileTheory.OLEAST_EQ_SOME] >>
+ metis_tac [weak_exec_exists, weak_exec_to_n]
+) >>
+(* Suppose there exists some earlier encounter of s''' *)
+Cases_on `?n_l''. n_l'' < (n_l' + 1) /\ weak_exec_n TS s ls n_l'' = SOME s'''` >- (
+ fs [whileTheory.OLEAST_EQ_SOME] >>
+ subgoal `weak_exec_n TS s''' ls (n_l - (n_l' + 1)) = SOME s'` >- (
+  irule weak_exec_n_split2 >>
+  fs [] >>
+  qexists_tac `s` >>
+  fs []
+ ) >>
+ subgoal `weak_exec_n TS s ls (n_l'' + (n_l - (n_l' + 1))) = SOME s'` >- (
+  irule weak_exec_n_add >>
+  fs [] >>
+  qexists_tac `s'3'` >>
+  fs []
+ ) >>
+ QSPECL_ASSUM ``!n. n < n_l ==> weak_exec_n TS s ls n <> SOME s'`` [`(n_l'' + (n_l - (n_l' + 1)))`] >>
+ gs []
+) >>
+fs [] >>
+(* If there were no earlier encounter of s''', then the first encounter was at n_l' + 1 *)
+subgoal `(OLEAST n_l. weak_exec_n TS s ls n_l = SOME s''') = SOME (n_l' + 1)` >- (
+ fs [whileTheory.OLEAST_EQ_SOME] >>
+ metis_tac []
+) >>
+
+(* Suppose there exists some later encounter of s''' *)
+Cases_on `?n_l''. n_l'' > (n_l' + 1) /\ n_l'' < n_l /\ weak_exec_n TS s ls n_l'' = SOME s'''` >- (
+ fs [] >>
+ subgoal `(OLEAST n_l. weak_exec_n TS s''' ls n_l = SOME s') = SOME (n_l - (n_l' + 1))` >- (
+  fs [whileTheory.OLEAST_EQ_SOME] >>
+  rpt strip_tac >| [
+   irule weak_exec_n_split2 >>
+   fs [] >>
+   qexists_tac `s` >>
+   fs [],
+
+   subgoal `weak_exec_n TS s ls ((n_l' + 1) + n_l'3') <> SOME s'` >- (
+    QSPECL_ASSUM ``!n. n < n_l ==> weak_exec_n TS s ls n <> SOME s'`` [`(n_l' + 1) + n_l'3'`] >>
+    gs []
+   ) >>
+   subgoal `weak_exec_n TS s ls ((n_l' + 1) + n_l'3') = SOME s'` >- (
+    irule weak_exec_n_add >>
+    fs []
+   )
+  ]
+ ) >>
+ subgoal `weak_exec_n TS s''' ls (n_l'' - (n_l' + 1)) = SOME s'''` >- (
+  irule weak_exec_n_split2 >>
+  fs [] >>
+  qexists_tac `s` >>
+  fs []
+ ) >>
+ (* By weak_exec_n_cycle *)
+ subgoal `(n_l - (n_l' + 1)) < (n_l'' - (n_l' + 1))` >- (
+  irule weak_exec_n_cycle >>
+  fs [] >>
+  qexistsl_tac [`TS`, `ls`, `s'''`, `s'`] >>
+  gs [whileTheory.OLEAST_EQ_SOME]
+ ) >>
+ gs []
+) >>
+fs [] >>
+gs [pred_setTheory.SING_DEF, GSYM pred_setTheory.UNIQUE_MEMBER_SING] >>
+qexists_tac `n_l' + 1` >>
+rpt strip_tac >| [
+ Cases_on `n_l' + 1 = n_l` >- (
+  gvs [whileTheory.OLEAST_EQ_SOME]
+ ) >>
+ gs [],
+
+ irule weak_exec_n_add >>
+ fs [] >>
+ qexists_tac `s''` >>
+ fs [whileTheory.OLEAST_EQ_SOME] >>
+ metis_tac [weak_exec_exists, weak_exec_to_n],
+
+ res_tac >>
+ gs [arithmeticTheory.EQ_LESS_EQ, arithmeticTheory.NOT_LESS]
+]
+QED
+
+Theorem weak_exec_unique_start:
+ !TS.
+ first_enc TS ==>
+ !s ls s' n_l. 
+ (OLEAST n. weak_exec_n TS s ls n = SOME s') = SOME n_l ==>
+ s <> s' ==>
+ SING (\n_l'. n_l' < n_l /\ weak_exec_n TS s ls n_l' = SOME s)
+Proof
+rpt strip_tac >>
+gs [pred_setTheory.SING_DEF, GSYM pred_setTheory.UNIQUE_MEMBER_SING] >>
+qexists_tac `0` >>
+rpt strip_tac >| [
+ Cases_on `n_l = 0` >> (
+  fs [weak_exec_n_def, FUNPOW_OPT_compute, whileTheory.OLEAST_EQ_SOME]
+ ),
+
+ fs [weak_exec_n_def, FUNPOW_OPT_compute],
+
+ Cases_on `y > 0` >- (
+  imp_res_tac weak_exec_n_cycle >>
+  fs []
+ ) >>
+ fs []
+]
+QED
+
+(* Uses the fact that exit labels are disjoint from loop point to know that
+ * we have not yet exited the loop after another weak transition, i.e. the
+ * number of loops is still less than n_l *)
+Theorem weak_exec_less_incr_superset:
+ !TS.
+  first_enc TS ==>
+   !ls1 ls2 s s' s'' s''' n_l n_l'.
+   DISJOINT ls1 ls2 ==>
+   (OLEAST n. weak_exec_n TS s (ls1 UNION ls2) n = SOME s') = SOME n_l ==>
+   TS.ctrl s' IN ls2 ==>
+   (OLEAST n. weak_exec_n TS s (ls1 UNION ls2) n = SOME s'') = SOME n_l' ==>
+   n_l' < n_l ==>
+   TS.weak (ls1 UNION ls2) s'' s''' ==>
+   TS.ctrl s''' NOTIN ls2 ==>
+   SUC n_l' < n_l
+Proof
+rpt strip_tac >>
+Cases_on `SUC n_l' = n_l` >- (
+ subgoal `s''' = s'` >- (
+  subgoal `weak_exec_n TS s (ls1 UNION ls2) (SUC n_l') = SOME s'''` >- (
+   metis_tac [weak_exec_incr_last]
+  ) >>
+  gs [whileTheory.OLEAST_EQ_SOME]
+ ) >>
+ fs []
+) >>
+fs []
+QED
+
+
+val _ = export_theory();
